coq/Compiler/CompilerModel/CompilerRuntime.v
@@ -16,7 +16,7 @@
 
 Require Import String.
 Require Import Utils BasicRuntime.
-Require Import ForeignToJava ForeignToJavascript ForeignToJSON ForeignTypeToJSON.
+Require Import ForeignToJava ForeignToJavascript ForeignToScala ForeignToJSON ForeignTypeToJSON.
 Require Import ForeignReduceOps ForeignToReduceOps.
 Require Import ForeignToSpark.
 Require Import ForeignCloudant ForeignToCloudant.
@@ -29,6 +29,7 @@ Module Type CompilerRuntime.
   Axiom compiler_foreign_runtime : foreign_runtime.
   Axiom compiler_foreign_to_java : foreign_to_java.
   Axiom compiler_foreign_to_javascript : foreign_to_javascript.
+  Axiom compiler_foreign_to_scala : foreign_to_scala.
   Axiom compiler_foreign_to_JSON : foreign_to_JSON.
   Axiom compiler_foreign_type_to_JSON : foreign_type_to_JSON.
   Axiom compiler_foreign_reduce_op : foreign_reduce_op.
